Working on pulling existentials. This does not compile

MirrorCharge!/src/ILPullQuant.v
@@ -22,6 +22,7 @@ Require Import ExtLib.Tactics.Injection.
 Require Import ExtLib.Tactics.EqDep.
 Require Import Ext.SetoidFold.
 Require Import Relation_Definitions.
+Require Import MirrorCore.Ext.AppFull.
 
 Set Implicit Arguments. 
 Unset Strict Implicit.
@@ -30,6 +31,458 @@ Set Maximal Implicit Insertion.
 Definition inhabited (ts : types)  := forall (t : typ),
   option (Inhabited (typD ts nil t)).
   
+Section PullQuant.
+  Context (ts : types) (funcs : fun_map ts) (gs : logic_ops ts).
+  Context {es : embed_ops ts}.
+
+  Definition TT := option (list typ * expr ilfunc)%type.
+
+  Local Instance RSym_sym : SymI.RSym (typD ts) ilfunc := RSym_ilfunc funcs gs es.
+
+  Let T := tenv typ -> tenv typ -> TT.
+  Definition atomic (e : expr ilfunc) : T := fun _ _ => Some (nil, e).
+
+  Definition pq_var (v : var) : T := atomic (Var v).
+  Definition pq_uvar (u : uvar) : T := atomic (UVar u).
+  Definition pq_inj (s : ilfunc) : T := atomic (Inj s).
+  Definition pq_abs (x : typ) (e : expr ilfunc) (t : T) : T := 
+    fun us vs => t us (x::vs).
+
+  Definition pq_app (f : expr ilfunc) (_ : T) (args : list (expr ilfunc * T)) : T :=
+    fun us vs =>
+    match f, args with
+      | Inj (ilf_true t), nil => (atomic f) us vs
+      | Inj (ilf_and t), (_, a)::(_, b)::nil =>
+        match a us vs, b us vs with
+          | Some (xs, a), Some (ys, b) => Some (xs ++ ys, App (App f a) (lift 0 (length xs) b))
+          | _, _                       => None
+        end
+      | Inj (ilf_exists x t), (_, f)::nil =>
+        match f us vs with
+          | Some (ys, f) => Some (x::ys, f) 
+          | _            => None
+        end
+      | _, _ => None
+    end.
+
+    Definition pqArgs : AppFullFoldArgs ilfunc TT :=
+      @Build_AppFullFoldArgs ilfunc TT pq_var pq_uvar pq_inj pq_abs pq_app.
+
+    Definition Teval (e : TT) (t : typ) :=
+      match e with
+          | Some (xs, a) => 
+            Some (fold_right (fun x a => App (Inj (ilf_exists x t)) 
+                                             (Abs x a)) a xs)
+          | None         => None
+      end.
+
+    Definition TD (t : typ) (e : TT) (us : env (typD ts)) (vs : tenv typ) :=
+      match Teval e t with
+        | Some e => exprD' us vs e t
+        | None   => None
+      end.
+
+    Definition Ttype (ts us : tenv typ) (e : TT) (t : typ) :=
+      match Teval e t with
+        | Some e => typeof_expr ts us e
+        | None   => None
+      end.
+
+    Definition PQtype (e : expr ilfunc) (tt : TT) (us vs : tenv typ) :=
+      match typeof_expr us vs e with
+        | Some t => 
+          match Ttype us vs tt t with
+            | Some t' => t ?[eq] t' = true
+            | None    => True
+          end
+        | None => True
+      end.
+
+    Definition PQR (t : typ) {HIL : ILogicOps (typD ts nil t)} (e : expr ilfunc) (arg : TT) (us : env (typD ts)) (vs : tenv typ) :=
+      match TD t arg us vs, exprD' us vs e t with
+        | None, _ => True
+        | Some p, Some q => forall vs, (p vs) |-- (q vs)
+        | _, _ => False
+      end.
+
+  Lemma Habs
+    : forall tus tvs t t' e e_res {HIL : ILogicOps (typD ts nil t')} {HIL' : ILogicOps (typD ts nil (tyArr t t'))},
+        typeof_expr (typeof_env tus) tvs (Abs t e) = Some (tyArr t t') ->
+        @PQR t' _ e (e_res (typeof_env tus) (t :: tvs)) tus (t :: tvs) ->
+        @PQR (tyArr t t') HIL' (Abs t e) (pq_abs t e e_res (typeof_env tus) tvs) tus tvs.
+  Proof.
+    intros.
+    unfold PQR, pq_abs in *; simpl in *.
+    remember (exprD' tus tvs (Abs t e) (tyArr t t')) as o; destruct o.
+    rewrite exprD'_Abs in Heqo. rewrite typ_cast_typ_refl in Heqo.
+    remember (exprD' tus (t :: tvs) e t') as o; destruct o; [|inversion Heqo].
+    inv_all; subst.
+    unfold TD, Teval in *; simpl in *.
+    remember (e_res (typeof_env tus) (t :: tvs)) as o; destruct o; [|apply I].
+    destruct p; simpl in *.
+    induction l; simpl in *.
+
+    SearchAbout exprD' tyArr.
+    red_exprD.
+    admit.
+
+    Lemma Hatomic
+    : forall tus tvs v,
+            PQtype (Var v) (pq_var v tus tvs) tus tvs
+        /\ forall us vs,
+             WellTyped_env tus us ->
+             WellTyped_env tvs vs ->
+             PQR (Var v) (pq_var v tus tvs) us vs.
+    Proof.
+      intros.
+      split.
+      unfold PQtype, pq_var, atomic, Ttype.
+      simpl.
+      remember (nth_error tvs v).
+      destruct e; [apply rel_dec_correct; reflexivity | apply I].
+      intros.
+      unfold PQR. simpl.
+      remember (nth_error (typeof_env vs) v).
+      destruct e; [|apply I].
+
+      unfold TD. remember (Teval (pq_var v tus tvs) t) as o; destruct o.
+      simpl in *. inv_all; subst. reflexivity.
+      simpl in *. inversion Heqo.
+    Qed.
+(*
+      Lemma typeof_expr_fold_cons uvs t t' vvs (f : typ -> expr ilfunc -> typ -> expr ilfunc) (e : expr ilfunc) l
+            (H : typeof_expr uvs (t::vvs) (fold_right (fun x e => f x e t') e l) = Some t') :
+            typeof_expr uvs vvs (fold_right (fun x e => f x e (tyArr t t')) e l) = Some (tyArr t t').
+        induction l; simpl in *.
+        induction e; simpl in *.
+*)
+
+    Lemma typeof_expr_apps uvs vvs e lst (H: typeof_expr uvs vvs e = None) :
+      typeof_expr uvs vvs (apps e lst) = None.
+    Proof.
+      generalize dependent e; induction lst; intros; simpl.
+      + apply H.
+      + apply IHlst; simpl; rewrite H; reflexivity.
+    Qed.
+
+    Ltac PQtype_elim :=
+    match goal with 
+      | |- match ?o with | Some _ => _ | None => True end => destruct o; apply I
+    end.
+
+    Lemma Happ
+    : forall tus tvs l l_res rs,
+        PQtype l (l_res tus tvs) tus tvs ->
+        List.Forall (fun x => PQtype (fst x) (snd x tus tvs) tus tvs) rs ->
+           PQtype (apps l (map fst rs)) (pq_app l l_res rs tus tvs) tus tvs
+        /\ forall us vs,
+             PQR l (l_res tus tvs) us vs ->
+             List.Forall (fun x => PQR (fst x) (snd x tus tvs) us vs) rs ->
+             PQR (apps l (map fst rs))
+                 (pq_app l l_res rs tus tvs)
+                 us vs.
+      Proof.
+        intros; split.
+        + unfold PQtype in *.
+          remember (typeof_expr tus tvs l) as o; destruct o.
+          - destruct l; simpl; try PQtype_elim.
+            destruct i; simpl; try PQtype_elim.
+            * destruct rs; simpl; try PQtype_elim.
+              remember (gs t0) as o; destruct o; [|apply I].
+              unfold atomic, Ttype; simpl. rewrite <- Heqo0.
+              apply rel_dec_correct. reflexivity.
+            * destruct rs; simpl; try PQtype_elim.
+              destruct p; simpl in *.
+              destruct rs; simpl; try PQtype_elim. 
+              destruct p; simpl in *.
+              destruct rs; simpl; try PQtype_elim.
+              destruct (gs t0); [|apply I].
+              inv_all; subst.
+              simpl.
+              inversion H0; subst; clear H0.
+              inversion H4; subst; clear H4.
+              simpl in *. clear H5.
+              remember (typeof_expr tus tvs e) as o; destruct o; [|apply I].
+              remember (typ_eqb t0 t) as b; destruct b; [|apply I].
+              remember (typeof_expr tus tvs e0) as o; destruct o; [|apply I].
+              simpl. 
+              remember (typ_eqb t0 t3) as b; destruct b; [|apply I].
+              remember (t1 tus tvs) as o; destruct o; [|apply I]; destruct p; simpl.
+              remember (t2 tus tvs) as o; destruct o; [|apply I]; destruct p; simpl.
+              remember (Ttype tus tvs
+                              (Some
+                                 (l ++ l0, App (App (Inj (ilf_and t0)) e1) 
+                                               (lift 0 (length l) e2)))
+                              t0) as o; destruct o; [|apply I].
+              symmetry in Heqb; symmetry in Heqb0.
+              apply typ_eqb_true in Heqb; apply typ_eqb_true in Heqb0; do 2 subst.
+              clear -Heqo3 Heqo Heqo0.
+              induction l. simpl in *.
+              induction l0; simpl in *.
+              unfold Ttype in *; simpl in *.
+              destruct (gs t3); [|congruence].
+              rewrite <- Heqo0.
+              admit.
+              remember (t2 tus tvs) as o; destruct o; [|apply I]; destruct p; simpl.
+              simpl.
+              Set Printing All.
+              rewrite <- Heqo1.
+              admit.
+              remember (typ_eqb t0 tx) as b; destruct b.
+inversion H0; subst. destruct p; simpl in *.
+              
+            simpl.
+            remember (typeof_expr tus tvs (apps (Var v) (map fst rs))) as o; destruct o; apply I.
+            admit.
+            intuition.
+            unfold Ttype; simpl.
+            remember (map fst rs).clear Heql.
+            destruct rs; simpl in *.
+
+             Print List.Forall.
+            induction l. simpl.
+            simpl.
+          - rewrite typeof_expr_apps; intuition.
+          
+          Eval compute in apps (Var 0) (Var 1::Var 2::Var 3::nil).
+
+        unfold PQtype in *; destruct l; simpl.
+        destruct rs. simpl.
+        admit. simpl. destruct p; simpl.
+        unfold apps. simpl.
+        unfold pq_app.
+        destruct l.
+        split.
+Print apps.
+        unfold PQtype in *.
+        simpl in *.
+        unfold PQtype in *.v
+
+    Lemma Habs : forall tus tvs t e e_res,
+        PQtype e (e_res tus (t :: tvs)) tus (t :: tvs) ->
+           PQtype (Abs t e) (pq_abs t e e_res tus tvs) tus tvs
+        /\ forall us vs,
+             WellTyped_env tus us ->
+             WellTyped_env tvs vs ->
+             (forall x,
+                PQR e (e_res tus (t :: tvs)) us (@existT _ _ t x :: vs)) ->
+             PQR (Abs t e) (pq_abs t e e_res tus tvs) us vs.
+    Proof.
+      intros.
+      split.
+      unfold PQtype, pq_abs in *.
+      simpl. remember (typeof_expr tus (t :: tvs) e) as o; destruct o; [|apply I].
+      unfold Ttype, Teval in *; simpl in *.
+      remember (e_res tus (t :: tvs)) as o; destruct o; [|destruct H].
+      destruct p.
+      
+      
+      remember (typeof_expr tus (t::tvs) (fold_right
+          (fun (x : typ) (a : expr ilfunc) =>
+           App (Inj (ilf_exists x t0)) (Abs x a)) e0 l)) as o.
+      destruct o; [|destruct H].
+
+
+Print typeof_expr.
+        simpl.
+
+      SearchAbout typeof_expr.
+      pose proof (typeof_expr_lift RSym_sym tus nil (t::nil) tvs
+                                   ((fold_right
+               (fun (x : typ) (a : expr ilfunc) =>
+                App (Inj (ilf_exists x (tyArr t t0))) (Abs x a)) e0 l))).
+      simpl in H0. rewrite <- H0. clear H0.
+      
+      
+      remember 
+      admit.
+      forward.
+      simpl in *.
+      simpl.
+      
+
+      remember (typeof_expr tus tvs (Abs t e)) as o; destruct o; [|apply I].
+      simpl in *.
+      red_exprD.
+
+
+
+    Lemma Hatomic : forall us tvs t e val,
+                   exprD' us tvs e t = Some val ->
+                   forall vs,
+                     @PQR t (val vs) (atomic e (typeof_env us) tvs) us (join_env vs).    
+    Proof.
+      intros; unfold PQR; simpl. 
+      match goal with 
+        | |- ?x = _ => let x' := eval red in x in change x with x'
+      end;
+      rewrite split_env_join_env, H; reflexivity.
+    Qed.
+
+    Definition PQvar us tvs t v val := @Hatomic us tvs t (Var v) val.
+    Definition PQuvar us tvs t u val := @Hatomic us tvs t (UVar u) val.
+    Definition PQinj us tvs t i val := @Hatomic us tvs t (Inj i) val.
+
+    Require Import ExtLib.Data.HList.
+
+    Lemma PQabs : forall us tvs t t' e e_res val,
+                        exprD' us (t :: tvs) e t' = Some val ->
+                        forall (vs : hlist (typD ts nil) tvs),
+                          (forall x,
+                             @PQR t' (val (Hcons x vs)) (e_res (typeof_env us) (t :: tvs))
+                               us ((@existT _ (typD ts nil) t x) :: join_env vs)) ->
+                          @PQR (tyArr t t') (fun x => val (Hcons x vs))
+                            (pq_abs t e e_res (typeof_env us) tvs) us (join_env vs).
+    Proof.
+      intros.
+      unfold PQR, TD, pq_abs in *.
+
+      forward.
+      SearchAbout exprD' cons.
+      simpl in *. unfold pq_abs.
+      assert (tvs <> nil). {
+        intros Htvs.
+        remember (e_res (typeof_env us) (t :: tvs)) as o.
+        destruct o; simpl in *.
+        admit.
+        rewrite Htvs in *.        
+      }.
+      assert (~(length tvs = 0)). {
+        intro Htvs.
+        assert (tvs = nil).
+      assert (length tvs > 0).
+      destruct o; simpl in *; try congruence.
+      destruct p; simpl in *.
+      admit. 
+      Check e_res.
+      unfold e_res in Heqo.
+      Print 
+specialize (
+      forward.
+    Qed.
+
+    Lemma PQapp
+    : forall us tvs l l_res (rs : list (expr ilfunc * T)) t
+             (tvals : list {t : typ & hlist (typD ts nil) tvs -> typD ts nil t}) val,
+        exprD' us tvs l (fold_left (fun x y => tyArr y x) (map (@projT1 _ _) tvals) t) = Some val ->
+        Forall2 (fun e tval => exprD' us tvs (fst e) (projT1 tval) = Some (projT2 tval))
+                rs
+                tvals ->
+        forall vs : hlist (typD ts nil) tvs,
+          @PQR (fold_left (fun x y => tyArr y x) (map (@projT1 _ _) tvals) t)
+             (val vs) (l_res (typeof_env us) tvs) us (join_env vs) ->
+          Forall2 (fun x (t : {t : typ & hlist (typD ts nil) tvs -> typD ts nil t}) =>
+                     @PQR (projT1 t) (projT2 t vs) (snd x (typeof_env us) tvs) us (join_env vs))
+                  rs
+                  tvals ->
+          @PQR t (@apply ts _ vs tvals t (val vs))
+             (pq_app l l_res rs (typeof_env us) tvs)
+             us (join_env vs).
+    Proof.
+      admit.
+    Qed.
+
+      Check @semArgsOk ts ilfunc RSym_sym TT pq_var pq_uvar pq_inj pq_abs pq_app (@PQR)
+            (@PQvar) (@PQuvar) (@PQinj) (@PQabs) (@PQapp).
+
+
+End PullQuant.
+
+Section TestPullQuant.
+
+  Context {A : Type} {ILO : ILogicOps A}.
+
+  Context (logics_sound : forall g, match logics g with
+                                  | Some T => @ILogic _ T
+                                  | None => unit
+                                end).
+
+  Variable eq_nat : nat -> nat -> A.
+  Definition ts : types := (default_type A)::(default_type nat)::nil.
+  Variable es : embed_ops ts.
+  Variable funcs : fun_map ts.
+  Definition logics : logic_ops ts :=
+    fun t => match t with
+               | tyType 0 => Some ILO
+               | tyProp => Some _
+               | _ => None
+             end.
+
+  Definition test_fold := fun x => TD (es := es) (funcs) logics (tyType 0) (app_fold_args pqArgs x nil nil).
+
+  Eval cbv - [land ltrue lexists] in test_fold inj_true nil nil.
+  Eval cbv - [land ltrue lexists] in test_fold (inj_and inj_true inj_true) nil nil.
+  Eval cbv - [land ltrue lexists] in test_fold
+                   (inj_and (inj_exists (tyType 1) (inj_and inj_true (inj_exists (tyType 1) inj_true))) inj_true) nil nil.
+  Eval cbv - [land ltrue lexists] in test_fold
+                   (inj_and (inj_exists (tyType 0) (Var 0)) (inj_exists (tyType 0) (Var 0))) nil nil.
+ Eval cbv - [land ltrue lexists] in test_fold
+                   (inj_exists (tyType 1)
+                                        (inj_exists (tyType 0) (Var 0))) nil nil.
+  Eval compute in test_fold
+                   (inj_and (inj_exists (tyType 1) (inj_and inj_true
+                                                            (inj_exists (tyType 2) (Var 0))))
+                            inj_true) nil nil.
+Print inj_exists.
+Definition test_fold := @setoid_fold _ _ _ (atomic (SRW_Algo_pull_quant logics)) (SetoidFold.app (SRW_Algo_pull_quant logics))
+                   (SetoidFold.abs (SRW_Algo_pull_quant logics)) nil nil.
+
+Eval compute in test_fold (Abs (tyType 1) inj_true) (Rpointwise (tyType 1) (Rinj ent)).
+Eval compute in test_fold (Inj (ilf_exists (tyType 1) (tyType 0))) (Rfunctorial (Rpointwise (tyType 1) (Rinj ent)) (Rinj ent)).
+
+
+
+Eval compute in 
+  Eval compute in
+      @setoid_fold _ _ _ (atomic SRW_Algo_pull_quant) (SetoidFold.app SRW_Algo_pull_quant)
+                   (SetoidFold.abs SRW_Algo_pull_quant) nil nil 
+                   (inj_and (inj_exists (tyType 1) (inj_eq_nat (Var 0) (Var 0))) inj_true) 
+                   (Rinj ent).
+  simpl.
+Check @setoid_fold.
+  Eval compute in
+      @setoid_fold _ _ _ _ _ properAt atomic app nil (Inj And) (tyProp :: nil)
+                      (PRfunctorial (PRguess _ tyProp) (PRfunctorial (PRguess _ tyProp) (PRinj Impl))).
+
+End TestPullQuant.
+
+    Variable TT : Type.
+    Let T := tenv typ -> tenv typ -> TT.
+
+    Variable do_var : var -> T.
+    Variable do_uvar : uvar -> T.
+    Variable do_inj : sym -> T.
+    Variable do_abs : typ -> expr sym -> T -> T.
+    Variable do_app : expr sym -> T ->
+                      list (expr sym * T) -> T.
+
+    Definition semArgs : AppFullFoldArgs TT :=
+      @Build_AppFullFoldArgs TT do_var do_uvar do_inj do_abs do_app.
+
+    Variable R : forall t, typD ts nil t -> TT -> env (typD ts) -> env (typD ts) -> Prop.
+    Hypothesis Hvar : forall us tvs t v val,
+                        exprD' us tvs (Var v) t = Some val ->
+                        forall vs,
+                          R t (val vs) (do_var v (typeof_env us) tvs) us (join_env vs).
+    Hypothesis Huvar : forall us tvs t v val,
+                        exprD' us tvs (UVar v) t = Some val ->
+                        forall vs,
+                          R t (val vs) (do_uvar v (typeof_env us) tvs) us (join_env vs).
+    Hypothesis Hinj : forall us tvs t v val,
+                        exprD' us tvs (Inj v) t = Some val ->
+                        forall vs,
+                          R t (val vs) (do_inj v (typeof_env us) tvs) us (join_env vs).
+    (** INTERESTING ONES **)
+    Hypothesis Habs : forall us tvs t t' e e_res val,
+                        exprD' us (t :: tvs) e t' = Some val ->
+                        forall (vs : hlist (typD ts nil) tvs),
+                          (forall x,
+                             R t' (val (Hcons x vs)) (e_res (typeof_env us) (t :: tvs))
+                               us ((@existT _ (typD ts nil) t x) :: join_env vs)) ->
+                          R (tyArr t t') (fun x => val (Hcons x vs))
+                            (do_abs t e e_res (typeof_env us) tvs) us (join_env vs).
+
+
 Section Relation.
 	Variable ts : types.
 	Variable func : Type.
@@ -70,14 +523,30 @@ Section PullExistsLeft.
   Local Instance RSym_sym : SymI.RSym (typD ts) ilfunc := RSym_ilfunc ts funcs gs.
 
   Variable us vs : env (typD ts).                       
-  Definition T := (list type * list typ * expr ilfunc)%type.
+  Definition T := (list typ * list typ * expr ilfunc)%type.
 
   Definition T_union (p q : T) : T :=
-  	(fst (fst p) ++ fst (fst q), snd (fst p) ++ snd (fst q),
-         App (lift 0 (length (fst (fst q))) (snd p)) (snd q)).
+    match p, q with
+        (a1, b1, c1), (a2, b2, c2) =>
+        (a1 ++ a2, b1 ++ b2, App (lift 0 ((length a2) + (length b2)) c1) c2)
+    end.
 
-  Definition T_to_expr (t : T) (il : typ) := 
-    fold_right (fun t e => App (Inj (ilf_exists t il)) (Abs t e)) (snd t) (fst t).
+  Fixpoint T_to_expr_aux (vs qs : list typ) e t :=
+    match vs, t with
+      | nil, _ => Some (fold_right (fun v e => App (Inj (ilf_exists v t)) (Abs v e)) 
+                                   e qs)
+      | v::vs, tyArr a t => 
+        match T_to_expr_aux vs qs e t, v ?[eq] a with
+          | Some x, true => Some (Abs a x)
+          | _, _ => None
+        end
+      | _, _ => None
+    end.
+
+  Definition T_to_expr (e : T) (t : typ) :=
+    match e with
+        (vs, qs, e) => T_to_expr_aux vs qs e t
+    end.
 
   Inductive Rbase := 
     | Ent t : (exists v, gs' ts gs t = Some v) -> Rbase
@@ -100,14 +569,21 @@ Section PullExistsLeft.
 
   Definition app (vs us : tenv typ) (pq p : T) (rpq rp : R Rbase) : option T := 
     match rpq with
-      | Rinj (Ent t _) =>
-        Some (fst pq ++ fst p, App (lift 0 (length (fst p)) (snd pq)) (snd p))
-      | Rpointwise t (Ent t' _) => 
+      | Rinj (Ent t _) => Some (T_union pq p)
+      | Rpointwise a (Rinj (Ent t _)) => 
+        match pq, p with
+          | ((tyArr a' t')::nil, a''::nil, Var 1), (a'''::ls, es, p) =>
+            if a' ?[eq] a'' && a'' ?[eq] a''' then
+              Some (ls, a''::es, p)
+            else
+              None
+          | _, _ => None
+        end
       | _ => None
     end.
 
   Definition abs (vs us : tenv typ) (t : typ) (p : T) (r : R Rbase) : option T :=
-    Some (t :: fst p, snd p).
+    Some (t :: fst (fst p), snd (fst p), snd p).
 
   Fixpoint unify (r : R Rbase) (p : PR Rbase) : bool :=
     match p with
@@ -178,9 +654,169 @@ Section PullExistsLeft.
       apply Ins_point. apply IHr'; intuition.
   Qed.
 
-  Definition atom (us vs : tenv typ) (e : expr ilfunc) (r : R Rbase) : option T := Some (nil, e).
+  Definition atom (us vs : tenv typ) (e : expr ilfunc) (r : R Rbase) : option T := 
+    match e with
+      | Inj (ilf_exists a t) => Some ((tyArr a t)::nil, a::nil, Var 1)
+      | _ => Some (nil, nil, e)
+    end.
 
-  Definition TD us vs (t : T) (il : typ) := exprD us vs (T_to_expr t il) il.
+  Lemma atom_cases (tus tvs : tenv typ) (e : expr ilfunc) (r : R Rbase) (res : T) 
+    (H : atom tus tvs e r = Some res) : 
+    (exists a t, (e = Inj (ilf_exists a t) /\ (res =  ((tyArr a t)::nil, a::nil, Var 1)))) \/
+    (res = (nil, nil, e)).
+  Proof.
+    destruct e; simpl in *; try (right; congruence).
+    destruct i; simpl in *; try (right; congruence).
+    left. exists t; exists t0. intuition congruence.
+  Qed.
+
+  Definition TD us vs (e : T) (t : typ) :=
+    match (T_to_expr e t) with
+      | Some x => exprD' us vs x t
+      | None   => None
+    end.
+ 
+
+  Require Import FunctionalExtensionality.
+
+  Lemma TD_abs uvs vvs avs a b c t x
+    (H : TD uvs vvs (a::avs, b, c) t = Some x) :
+      exists x, t = tyArr a x.
+  Proof.
+    unfold TD in H.
+    destruct t; simpl in *; try congruence.
+    forward; inv_all; subst. exists t2. reflexivity.
+  Qed.
+      
+  Lemma TD_abs_list uvs vvs avs b c t x
+    (H : TD uvs vvs (avs, b, c) t = Some x) :
+      exists y, t = fold_right tyArr y avs.
+  Proof.
+    generalize dependent t; generalize dependent vvs.
+    induction avs; intros; simpl in *.
+    + exists t; reflexivity.
+    + unfold TD, T_to_expr in H; simpl.
+      red_exprD; forward; inv_all; subst.
+      unfold TD, T_to_expr in IHavs.
+      red_exprD; forward; inv_all; subst.
+      specialize (IHavs _ _ t). rewrite H0 in IHavs.
+      destruct (IHavs H1) as [y Hy].
+      exists y. rewrite Hy. reflexivity.
+  Qed.
+
+  Lemma TD_abs_sem uvs vvs avs a b c t x :
+    TD uvs vvs (a::avs, b, c) (tyArr a t) = Some x <->
+    TD uvs (a::vvs) (avs, b, c) t = Some (fun g => x (HList.hlist_tl g) (HList.hlist_hd g)).
+  Proof.
+    split; intro H.
+    + unfold TD, T_to_expr in H; simpl in H.
+      red_exprD; forward; inv_all; subst.
+      red_exprD; forward; inv_all; subst.
+      rewrite x0.
+      unfold TD, T_to_expr. rewrite H. rewrite H2.
+      f_equal. apply functional_extensionality; intros x.
+      rewrite <- HList.hlist_cons_eta. reflexivity.
+    + unfold TD, T_to_expr in *; simpl in *.
+      forward. red_exprD; forward. inv_all; subst.
+      rewrite typ_cast_typ_refl.
+      f_equal. 
+  Qed.
+
+  Fixpoint typD_fold_right tvs uvs t avs :
+    typD tvs uvs (fold_right tyArr t avs) -> HList.hlist (typD tvs uvs) avs ->
+    typD tvs uvs t :=
+    match avs with
+      | nil => fun x _ => x
+      | a::avs => fun f lst => typD_fold_right (f (HList.hlist_hd lst)) (HList.hlist_tl lst)
+    end.
+(*
+  Lemma TD_abs_list_sem uvs vvs avs b c t x :
+    (TD uvs vvs (avs, b, c) (fold_right tyArr t avs) = Some x) <->
+    TD uvs ((rev avs) ++ vvs) (nil, b, c) t = 
+    Some (fun g => match HList.hlist_split (rev avs) vvs g with
+                     | (a, b) => typD_fold_right (x b) a
+                   end).
+  Proof.
+    split; intro H.
+    + generalize dependent t; generalize dependent vvs.
+      induction avs; simpl in *; intros. 
+      * rewrite H. f_equal.
+      * apply TD_abs_sem in H.
+        apply IHavs in H.
+        admit.
+    + generalize dependent t; generalize dependent vvs.
+      induction avs; simpl in *; intros.
+      * rewrite H. reflexivity.
+      * admit.
+  Qed.
+*)
+  
+  Lemma TD_quant_sem_aux uvs vvs e t a (v : typD ts nil a) x :
+    TD uvs (a::vvs) e t = Some x <->
+    TD uvs vvs e t = Some (fun vs => x (HList.Hcons v vs)).
+  Proof.
+    split; intro H.
+    + unfold TD in *; simpl in *; forward.
+      pose proof (exprD'_lower RSym_sym us nil (a::nil) vvs e0).
+      simpl in *.
+      
+      red_exprD.
+      forward.
+      pose proof (exprD'_lift RSym_sym us nil (a::nil) vvs e0 t).
+      
+      simpl in *.
+      SearchAbout lift.
+    simpl.
+    
+    
+
+
+  Lemma TD_quant_sem_aux uvs vvs q qs c t x IL (a : typD ts nil q)
+        (HIL : gs' ts gs t = Some IL)
+        (H : TD uvs vvs (nil, q::qs, c) t = Some x) :
+        exists f, x = (fun vs => lexists (f vs)) /\
+                    TD uvs vvs (nil, qs, c) t = Some (fun vs => f vs a).
+  Proof.
+    unfold TD, T_to_expr in *; simpl in H.
+    red_exprD; forward; inv_all; revert H4; generalize dependent t2; subst; intros.
+    destruct x0. subst.
+    red_exprD; forward; inv_all; subst.
+    simpl in *. forward; inv_all; subst.
+    exists (fun x a => t (HList.Hcons a x)).
+    split. simpl. 
+    apply functional_extensionality; intros x1; simpl.
+    uip_all. reflexivity.
+    rewrite H2.
+    destruct x0.
+rewrite <- H7 in H5.
+rewrite <- H7 in x0. rewrite H7 in H5.
+    red_exprD; forward; inv_all; uip_all.
+    rewrite HIL in *. rewrite <- H6 in *. rewrite H7 in *. rewrite x0 in *. 
+    red_exprD; forward; inv_all. simpl in *. forward. inv_all.
+    red_exprD; forward; inv_all; revert H4; generalize dependent t2; subst; intros.
+    rewrite typ_cast_typ_refl in H2.
+    simpl.
+    red_exprD; forward; inv_all.
+    f_equal. generalize dependent t2; subst; intros.
+    apply functional_extensionality; intros; simpl.
+    red_exprD; forward; inv_all; subst; simpl in *.
+    f_equal. apply functional_extensionality. intros; simpl.
+    admit.
+  Qed.
+
+  Lemma TD_quant_sem uvs vvs q qs c il t f IL
+        (HIL : gs' ts gs t = Some IL)
+        (H : TD uvs (q::vvs) (nil, qs, c) il t = Some f) :
+    TD uvs vvs (nil, qs, c) il t = Some (fun g => lexists (fun x => f (HList.Hcons x g))).
+  Proof.
+    unfold TD, T_to_expr in *.
+    simpl in *. remember ((fold_right
+           (fun (t : typ) (e : expr ilfunc) =>
+            App (Inj (ilf_exists t il)) (Abs t e)) c qs)) as y.
+    admit.
+  Qed.
+
+  
 
   Fixpoint RD (r : R Rbase) : (typD ts nil (typeForR typeForRbase r)) -> 
                               (typD ts nil (typeForR typeForRbase r)) -> Prop :=
@@ -207,8 +843,140 @@ Section PullExistsLeft.
   Qed.
 
   Definition TR us vs (r : R Rbase) (t : T) v : Prop :=
-    exists v', TD us vs t (typeForR typeForRbase r) = Some v' /\ @RD r v v'.
-(*
+    match TD us vs t (typeForR typeForRbase r) with 
+      | Some x => forall vs, @RD r v (x vs)
+      | None => False
+    end.
+
+  Theorem Happ
+  : forall us vs t1 t2 r1 r2 v1 v2 f result,
+      app (typeof_env us) (typeof_env vs) r1 r2 t1 t2 = Some result ->
+      exprD us vs f (typeForR typeForRbase (Rfunctorial t1 t2)) = Some v1 ->
+      @TR us (typeof_env vs) (Rfunctorial t1 t2) r1 v1 ->
+      @TR us (typeof_env vs) t1 r2 v2 ->
+      @TR us (typeof_env vs) t2 result (v1 v2).
+  Proof.
+    intros. simpl in *.
+    destruct r1 as [[rv1 re1] r1], r2 as [[rv2 re2] r2]; simpl in *.
+    unfold TR in *.
+    forward. simpl in *.
+Check TD.
+    (f : typD ts nil r -> 
+     (H: TD us0 (typeof_env vs0) (r::rv1, re1, r1)
+         (tyArr ) =
+       Some t0)
+       TD us0 (typeof_env vs0) (rv1, re1, r1)
+         (tyArr (typeForR typeForRbase t1) (typeForR typeForRbase t2)) =
+       Some f
+
+    unfold TD in H1.
+
+    
+
+    destruct t1; simpl in *; try congruence.
+    destruct r; simpl in *; try congruence.
+    inv_all; subst. unfold T_union; simpl.
+    unfold TR, TD, T_to_expr. simpl.
+    forward.
+    induction rv1. simpl. admit.
+    simpl in *.
+Eval compute in (typD ts nil (typeForR typeForRbase (Rpointwise a t2))).
+    Lemma TR_abs t uvs vvs r a rvs es p (v : typD ts nil (typeForR typeForRbase t))
+      (H : forall (x : typD ts nil a), exists f rd, f x = v /\ rd = Rpointwise a r /\ @TR uvs vvs (Rpointwise a r) (rvs, es, p) f) :
+      @TR uvs vvs r (a :: rvs, es, p) v.
+    Proof.
+      admit.
+    Qed.
+
+    apply TR_abs.
+    intros.
+
+    apply TR_abs. apply IHrv1.
+
+    inv_all; subst. unfold T_union; simpl.
+    unfold TR in *.
+    remember (TD us0 (typeof_env vs0) r1
+           (typeForR typeForRbase (Rfunctorial t1 t2))) as o.
+    destruct o; simpl in *; [|intuition].
+    remember (TD us0 (typeof_env vs0) r2 (typeForR typeForRbase t1)) as o.
+    destruct o; simpl in *; [|intuition].
+    destruct t1; simpl in *; try congruence.
+    destruct r; simpl in *; try congruence.
+    induction rv1. simpl. admit.
+    unfold TD, T_to_expr; simpl.
+    SearchAbout exprD' Abs.
+    red_exprD.
+    destruct t2; simpl in *; try congruence.
+    destruct r; simpl in *; try congruence.
+    destruct t2; simpl in *; try congruence.
+    unfold TD in IHrv1. simpl in *.
+    apply IHrv1.
+    remember (TD us0 (typeof_env vs0)
+       (a :: rv1 ++ rv2, re1 ++ re2,
+       App (lift 0 (length rv2 + length re2) r1) r2)
+       (typeForR typeForRbase t2)) as o.
+    destruct o; intros; simpl in *.
+    unfold TD, T_to_expr in Heqo.
+    simpl in Heqo.
+    red_exprD. forward.
+    unfold TR.
+    unfold TD.
+    unfold T_to_expr.
+    simpl.
+    unfold TR, TD, T_to_expr in H1; simpl in *.
+    unfold exprD in H1.
+    destruct vs0.
+    remember (exprD' us0 tvs
+            (Abs a
+               (fold_right Abs
+                  (fold_right
+                     (fun (t0 : typ) (e : expr ilfunc) =>
+                      App
+                        (Inj
+                           (ilf_exists t0
+                              (tyArr t (typeForR typeForRbase t2))))
+                        (Abs t0 e)) r1 re1) rv1))
+            (tyArr t (typeForR typeForRbase t2))).
+SearchAbout expr
+    red_exprD.
+    simpl in H1.
+    red_exprD.
+    simpl.
+    simpl.
+    
+    simpl.
+    simpl.
+
+destruct H1RD as [_ H1RD].
+    unfold app in H.
+    unfold TD, T_to_expr in *; simpl in *.
+    destruct t1; simpl in *; try congruence. 
+    destruct r; simpl in *; try congruence.
+    unfold TD in H1.
+    unfold app in H; simpl in *.
+    simpl in *.
+
+
+    Lemma TD_app us vs e1 e2 t1 t2 tr1 tr2 result
+          (H1 : TD us vs e1 (tyArr t1 t2) = Some tr1)
+          (H2 : TD us vs e2 t1 = Some tr2) 
+          (H3 : app (typeof_env us) (typeof_env vs) r1 r2 t1 t2 = Some result) :
+      TD us vs result t2 = Some (tr1 tr2).
+
+
+    unfold TD in *.
+    
+    specialize (H1RD _ _ H2RD). simpl in *.
+    simpl in *. 
+    unfold TR.
+    exists (v1 v2).
+    split; [|admit].
+    clear H1
+    red_exprD.
+    unfold TR.
+    unfold TD in *.
+    unfold T_to_expr in *.
+    simpl in *.
   Theorem Hatomic
     : forall tus tvs e r r' result,
         get_unified_proper  e r = Some r' ->
@@ -222,29 +990,96 @@ Section PullExistsLeft.
       remember (unify r0 r) as b; destruct b; congruence.
     + unfold get_unified_proper in H.
       remember (get_proper_aux e r) as o; destruct o; try congruence.
-      remember (unify r0 r) as b; destruct b; try congruence.
+      remember (unify r0 r) as b; destruct b; try congruence. 
       inv_all; subst.
-      clear H1; clear Heqb.
-      generalize dependent r'.
-      induction r; intros; simpl in *.
-      
-      
-  Lemma unification_type r r' t (H : unify r' r = true) 
-    (H1 : pr_type typeForRbase r t) : typeForR typeForRbase r' = t.
+      Print pr_type.
+  Lemma proper_lookup_type tus tvs e r r' r'' t 
+        (H : unify r' r = true) 
+        (H1 : proper_lookup e r'' = Some r')
+        (H2 : typeof_expr tus tvs e = Some t) :
+      typeForR typeForRbase r' = t.
   Proof.
-    generalize dependent r; induction r'; simpl; intros.
-    + destruct r0; try congruence.
-      - assert (r0 = r) by admit; subst. 
-        inversion H1; reflexivity.
-      - 
+    destruct e; simpl in *; try congruence;
+    destruct i; simpl in *; try congruence;
+    destruct r''; simpl in *; try congruence;
+    destruct e as [v ILV];
+    remember (t0 ?[ eq ] t1) as b;
+    destruct b; try congruence;
+    assert (t0 = t1) by admit; subst;
+    try rewrite ILV in H2; inv_all; subst; simpl; try reflexivity.
+    remember (t1 ?[eq] t2) as b.
+    destruct b; try congruence.
+    inv_all; subst; simpl in *.
+    destruct r; simpl in *; try congruence.
+    assert (t1 = t2) by admit; subst.
+    rewrite ILV in H2; inv_all.
+    assumption.
+    destruct r1; simpl in *; try congruence.
+    assert (t1 = t2) by admit; subst.
+    rewrite ILV in H2; inv_all.
+    destruct r2; simpl in *; try congruence. 
+    rewrite andb_true_iff in H; destruct H as [H H1].
+    rewrite andb_true_iff in H; destruct H as [H H0].
+    assert (t1 = t2) by admit; subst.
+    rewrite ILV in H2; inv_all. assumption.
+    admit.
   Qed.
- 
-Print pr_type.
+
+  Lemma unification_type tus tvs e r r' r'' t (H : unify r' r = true) 
+    (H1 : get_proper_aux e r'' = Some r') 
+    (H2 : pr_type typeForRbase r t) 
+    (H3 : typeof_expr tus tvs e = Some t) : typeForR typeForRbase r' = t.
+  Proof.
+    generalize dependent r; generalize dependent r'; induction r''; simpl; intros;
+    try congruence.
+    eapply proper_lookup_type; eauto.
+    eapply IHr''2; eauto.
+    eapply IHr''; eauto.
+  Qed.
+
+  
+  eapply unification_type; eauto. 
     + remember (exprD' us0 tvs e (typeForR typeForRbase r')).
       destruct o; [|apply I].
-      intros. unfold atom in H0. inversion H0; subst.
+      intros.
+      apply atom_cases in H0; destruct H0 as [[a [t1 [He Hres]]] | H0].
+      subst; unfold TR.
+      unfold TD, T_to_expr; simpl.
+      red_exprD; forward; inv_all; subst; simpl in *.
+      assert (exists IL, gs' ts gs t1 = Some IL) by admit.
+      destruct H4 as [IL H4].
+      rewrite H4 in H0. rewrite H4 in H2. inv_all; simpl in *.
+      subst; red_exprD. 
+      remember (typ_cast_typ ts nil (tyArr (tyArr a t1) t1)
+           (typeForR typeForRbase r')) as o.
+      destruct o; try congruence.
+      symmetry in Heqo. 
+      apply typ_cast_typ_eq in Heqo; subst.
+      exists t2.
+      split.
+      inv_all; subst.
+      unfold exprD. 
+      rewrite split_env_join_env.
+      red_exprD.
+      
+      uip_all.
+      rewrite <- Heqo.
+      simpl.
+      uip_all.
+      red_exprD.
+      simpl.
+      red_exprD.
+      eexists.
+
+Check typ_cast_typ_eq.
+rewrite typ_cast_typ_eq in Heqo.
+      SearchAbout typ_cast_typ.
+      red_exprD.
+      assert (t = tyArr (tyArr a t1) t1) by admit.
+      simpl.
+      subst.
       unfold TR.
-      clear H0. exists (t0 vs0).
+      exists (t0 vs0).
       split. unfold TD. simpl.
       unfold exprD; simpl.
       rewrite split_env_join_env.
@@ -253,7 +1088,7 @@ Print pr_type.
       destruct o; inv_all; subst; [reflexivity|congruence].
       apply RD_reflexive.
   Qed.
-*)
+
   Definition SRW_Algo_pull_quant := 
     @SRW_Algo_properAt ilfunc T Rbase get_unified_proper atom app abs.
                                                        
@@ -337,7 +1172,7 @@ Print setoid_fold_spec.
   Eval compute in
       @setoid_fold _ _ _ (atomic (SRW_Algo_pull_quant logics)) (SetoidFold.app (SRW_Algo_pull_quant logics))
                    (SetoidFold.abs (SRW_Algo_pull_quant logics)) nil nil
-                   (inj_exists (tyType 1) inj_true)
+                   (inj_and (inj_exists (tyType 1) (inj_and inj_true (inj_exists (tyType 2) inj_true))) inj_true)
                    (Rinj ent).
 
 Definition test_fold := @setoid_fold _ _ _ (atomic (SRW_Algo_pull_quant logics)) (SetoidFold.app (SRW_Algo_pull_quant logics))
